{
 "cells": [
  {
   "cell_type": "markdown",
   "metadata": {},
   "source": [
    "::Recurrence Relation::"
   ]
  },
  {
   "cell_type": "code",
   "execution_count": null,
   "metadata": {},
   "outputs": [],
   "source": [
    "#1. Find the value of T(2) for the recurrence relation T(n) = 3T(n-1) + 12n, given that T(0)=5\n",
    "\n",
    "\n",
    "'''\n",
    "    Given:\n",
    "    T(0)=5\n",
    "    \n",
    "    T(n) = 3T(n-1) + 12n ------(1)\n",
    "    \n",
    "    substuting eqn 1 by putting n = 1\n",
    "    \n",
    "    =  T(1) = 3T(1-1) + 12*1\n",
    "    =  T(1) = 3 * T(0) + 12\n",
    "    \n",
    "    Putting the given value of T(0)\n",
    "    =  T(1) = 3 * 5 + 12\n",
    "    =  T(1) = 27 -----------(2)\n",
    "    \n",
    "    Now substuting eqn 1 by putting n = 2\n",
    "    \n",
    "    =  T(2) = 3T(2-1) + 12*2\n",
    "    =  T(2) = 3 * T(1) + 24\n",
    "    \n",
    "     Putting the  value of T(2) from eqn 2\n",
    "     \n",
    "     T(2) = 3* 27 + 24\n",
    "     T(2) = 105 ---------------(3)\n",
    "     \n",
    "     \n",
    "     So from the eqn 3 ...We can see that the value of T(2) = 105\n",
    "     \n",
    "'''  \n",
    "\n",
    "    \n",
    "    \n",
    "\n"
   ]
  },
  {
   "cell_type": "code",
   "execution_count": 2,
   "metadata": {},
   "outputs": [
    {
     "data": {
      "text/plain": [
       "'\\n\\n    T(n) = T(n/2) +  c ------(1)\\n    \\n    Substitute n = n/2\\n    \\n    T(n/2) = T(n/2/2) +  c\\n    T(n/2) = T(n/4) +  c  -------(2)\\n    \\n    put the value of T(n/2) in eqn 1\\n    \\n    T(n) = T(n/2) +  c ------(1)\\n    T(n) = T(n/4) +  c) +  c \\n    T(n) = T(n/4) + 2c -------(3)\\n    \\n             |\\n            k times\\n             |\\n            \\n    From eqn 1 and 3 we can assume the kth term\\n    \\n    T(n) = T(n/(2**k)) + k.c ------(4)\\n    \\n    Now considerring base case n/(2**k) = 1\\n    \\n    n = 2**k\\n    log base2 of n=k\\n    \\n    Substitute the value of k in eqn 4\\n    \\n    T(n) = T(n/(2**(log base2 of n))) + (log base2 of n).c\\n    T(n) = T(1) + (log base2 of n).c\\n    \\n    As T(1) is a constant lets denote it as c base2\\n    \\n    T(n) = c base2 + (log base2 of n).c\\n    \\n    \\n    \\n    \\n    \\n    \\n'"
      ]
     },
     "execution_count": 2,
     "metadata": {},
     "output_type": "execute_result"
    }
   ],
   "source": [
    "#2. Given a recurrence relation, solve it using the substitution method:\n",
    "\n",
    "#a. T(n) = T(n-1) + c\n",
    "#b. T(n) = 2T(n/2) + n\n",
    "#c. T(n) = 2T(n/2) + c\n",
    "#d. T(n) = T(n/2) +  c\n",
    "\n",
    "\n",
    "#a. T(n) = T(n-1) + c\n",
    "'''\n",
    "    T(n) = T(n-1) + c --------(1)\n",
    "    \n",
    "    substitute by n = n-1 in eqn 1\n",
    "    \n",
    "    = T(n-1) = T((n-1)-1) + c\n",
    "    = T(n-1) = T(n-2) + c --------(2)\n",
    "    \n",
    "    Now put the value of T(n-1) in to eqn 1\n",
    "    \n",
    "    T(n) = T(n-2) + c + c\n",
    "    T(n) = T(n-2) + 2c ----------(3)\n",
    "    \n",
    "    Substitute the eqn 1 by n = n-2\n",
    "    \n",
    "    T(n-2) = T((n-2)-1) + c\n",
    "    T(n-2) = T(n-3) + c----------(4)\n",
    "    \n",
    "    Now put value of T(n-2) from eqn 4 in eqn 3\n",
    "    T(n) = T(n-2) + 2c\n",
    "    T(n) = T(n-3) + c + 2c\n",
    "    T(n) = T(n-3) + 3c------------(5)\n",
    "    \n",
    "                |\n",
    "            k times\n",
    "                |\n",
    "\n",
    "   From the above eqns 1, 3, 5 we can get a generalize\n",
    "   T(k) = T(n-k) + k.c\n",
    "   \n",
    "   According to base case we can assume that\n",
    "   =  n-k = 1\n",
    "   =  k = n-1 -----------(6)\n",
    "   \n",
    "    =T(n-k) + k.c\n",
    "    =T(n-(n-1)) + (n-1).c\n",
    "    =T(1) + (n-1).c\n",
    "    = 1 + (n-1).c--------(7)\n",
    "    \n",
    "    From eqn 7 we can assume that the time complexity will be O(n)\n",
    "    \n",
    "    So, Time complexity = O(n)\n",
    "    \n",
    "'''\n",
    "\n",
    "#b. T(n) = 2T(n/2) + n\n",
    "\n",
    "'''\n",
    "    T(n)=2T(n/2)+n ---------------(1)\n",
    "    \n",
    "    \n",
    "    Substitute n=n/2 in equation (1)\n",
    "\n",
    "    T(n/2)=2T(n/2/2)+n/2\n",
    "    T(n/2)=2T(n/4)+n/2 ---------------(2)\n",
    "\n",
    "    Now, put the value of \n",
    "\n",
    "    T(n/2) from equation (2) into equation (1)\n",
    "    \n",
    "    T(n)=2[2T(n/4)+n/2]+n\n",
    "\n",
    "    T(n)=4T(n/4)+2n\n",
    "    \n",
    "             |\n",
    "            k times\n",
    "             |\n",
    "\n",
    "    Continuing this process k times:\n",
    "\n",
    "    T(n)=2**k.T(n/2 k)+kn ---------------(3)\n",
    "\n",
    "    Now, n/2**k=1 (Considering the base case)\n",
    "\n",
    "    n=2**k\n",
    " \n",
    "    log base 2 n=k\n",
    "\n",
    "    Substitute the value of k in equation (3)\n",
    "    \n",
    "    T(n)=2**(log base2 n).T(1)+n log base2 n\n",
    "    T(n)=nT(1)+nlog2n\n",
    "    \n",
    "    As T(1) is a constant, let's denote it as c\n",
    "    T(n)=cn+nlog 2n\n",
    "    \n",
    "    So, Time complexity = O(n logn)\n",
    "'''\n",
    "\n",
    "#c. T(n) = 2T(n/2) + c\n",
    "\n",
    "'''\n",
    "    T(n) = 2T(n/2) + c -------(1)\n",
    "    \n",
    "    Substitute n = n/2\n",
    "    \n",
    "    T(n/2) = 2T(n/2/2) + c\n",
    "    T(n/2) = 2T(n/4) + c ------(2)\n",
    "    \n",
    "    From eqn 2 Put the value of T(n/2) in eqn 1\n",
    "    \n",
    "    T(n) = 2[2T(n/4) + c] + c\n",
    "    T(n) = 4T(n/4) + 2c + c\n",
    "    T(n) = 4T(n/4) + 3c -------(3)\n",
    "    \n",
    "             |\n",
    "            k times\n",
    "             |\n",
    "\n",
    "    Continuing this process k times\n",
    "    \n",
    "    T(n) = 2**k.T(n/(2**k)) + k.c -------(4)\n",
    "    \n",
    "    Now considerring base case n/(2**k) = 1\n",
    "    \n",
    "    n = 2**k\n",
    "    log base2 of n=k\n",
    "    \n",
    "    Substitute the value of k in eqn 4\n",
    "    \n",
    "    T(n) = 2**(log base2 of n).T(n/(2**(log base2 of n))) + (log base2 of n).c\n",
    "    \n",
    "    T(n) = nT(1) + n.c\n",
    "    \n",
    "    As T(1) is a constant, let's denote it as c base2\n",
    "    \n",
    "    T(n) = c base2 n + n.c\n",
    "    \n",
    "    So the time complexity is O(n)\n",
    "    \n",
    "'''\n",
    "#d. T(n) = T(n/2) +  c\n",
    "\n",
    "'''\n",
    "\n",
    "    T(n) = T(n/2) +  c ------(1)\n",
    "    \n",
    "    Substitute n = n/2\n",
    "    \n",
    "    T(n/2) = T(n/2/2) +  c\n",
    "    T(n/2) = T(n/4) +  c  -------(2)\n",
    "    \n",
    "    put the value of T(n/2) in eqn 1\n",
    "    \n",
    "    T(n) = T(n/2) +  c ------(1)\n",
    "    T(n) = T(n/4) +  c) +  c \n",
    "    T(n) = T(n/4) + 2c -------(3)\n",
    "    \n",
    "             |\n",
    "            k times\n",
    "             |\n",
    "            \n",
    "    From eqn 1 and 3 we can assume the kth term\n",
    "    \n",
    "    T(n) = T(n/(2**k)) + k.c ------(4)\n",
    "    \n",
    "    Now considerring base case n/(2**k) = 1\n",
    "    \n",
    "    n = 2**k\n",
    "    log base2 of n=k\n",
    "    \n",
    "    Substitute the value of k in eqn 4\n",
    "    \n",
    "    T(n) = T(n/(2**(log base2 of n))) + (log base2 of n).c\n",
    "    T(n) = T(1) + (log base2 of n).c\n",
    "    \n",
    "    As T(1) is a constant lets denote it as c base2\n",
    "    \n",
    "    T(n) = c base2 + (log base2 of n).c\n",
    "    \n",
    "    \n",
    "    So the Time Complexity is O(log n)\n",
    "    \n",
    "    \n",
    "    \n",
    "'''\n",
    "\n"
   ]
  },
  {
   "cell_type": "code",
   "execution_count": null,
   "metadata": {},
   "outputs": [],
   "source": [
    "\n",
    "#3. Given a recurrence relation, solve it %sing the recursive tree approach:\n",
    "    #a. T(n) = 2T(n-1) +1\n",
    "    #b. T(n) = 2T(n/2) + n\n",
    "    \n",
    "\n",
    "#a. T(n) = 2T(n-1) +1\n",
    "\n",
    "'''\n",
    "    Expanding T(n-1) in terms of T(n-2) and so on till base case\n",
    "    \n",
    "    T(n) = 2T(n-1) + 1\n",
    "         = 2[2T(n-2) + 1] + 1\n",
    "         = 2**2 T(n-2) + 2 + 1\n",
    "         = 2**2 [2T(n-3) + 1] + 2 + 1\n",
    "         = 2**3 T(n-3) + 2**2 + 2 + 1\n",
    "         \n",
    "         = 2**k T(n-k) + 2**0 + 2**1 + 2**2 +...+ 2**(k-1)\n",
    "         \n",
    "         When n-k = 1 \n",
    "         k = n-1\n",
    "         \n",
    "         T(n) = 2**n-1 T(1) + 2**0 + 2**1 + 2**2 + ...+ 2**n-2\n",
    "         \n",
    "         express the sum 2**0 + 2**1 + 2**2 + ...+ 2**n-2 as geometric series\n",
    "         \n",
    "         2**0 + 2**1 + 2**2 + ...+ 2**n-2 \n",
    "         \n",
    "         = (2**(n-1) - 1)/2-1\n",
    "         \n",
    "         = 2**(n-1) - 1\n",
    "         \n",
    "         Substituting back into eqn\n",
    "         T(n) = 2**(n-1) T(1) + (2**(n-1) - 1)\n",
    "         = 2**(n-1) T(1) + 2(n-1) - 1\n",
    "         \n",
    "         \n",
    "         So it could be exponential time complexity \n",
    "         approx O(2**n)\n",
    "    \n",
    "'''\n",
    "\n",
    "#b. T(n) = 2T(n/2) + n\n",
    "\n",
    "'''\n",
    "    Expand the recurrence relation we get\n",
    "   T(n) = 2T(n/2) + n\n",
    "   = 2[2T(n/4) + n/2] +n\n",
    "   = 2**2 T(n/4) + 2n/2 + n\n",
    "   = 2**2[2T(n/8) + n/4] + 2n/2 + n\n",
    "   = 2**3 T(n/8) + 3n/4 + n\n",
    "   \n",
    "   On both side of recurrsive approach we have addition of n\n",
    "   \n",
    "   expansion countinue till base case T(1) or T(2)\n",
    "   \n",
    "   As the division of n at each level (log n levels) and an addition of n at each step..\n",
    "   we determine that time complexity T(n) is O(n log n)\n",
    "\n",
    "\n",
    "\n",
    "'''\n",
    "\n"
   ]
  }
 ],
 "metadata": {
  "kernelspec": {
   "display_name": "Python 3 (ipykernel)",
   "language": "python",
   "name": "python3"
  },
  "language_info": {
   "codemirror_mode": {
    "name": "ipython",
    "version": 3
   },
   "file_extension": ".py",
   "mimetype": "text/x-python",
   "name": "python",
   "nbconvert_exporter": "python",
   "pygments_lexer": "ipython3",
   "version": "3.10.8"
  }
 },
 "nbformat": 4,
 "nbformat_minor": 4
}
